spanning.v
@@ -1,11 +1,10 @@
-From iris.algebra Require Import frac dec_agree gmap gset upred_big_op.
-From iris.program_logic Require Export invariants ghost_ownership.
-From iris.program_logic Require Import auth.
+From iris.algebra Require Import frac gmap gset excl.
+From iris.base_logic Require Export invariants.
 From iris.proofmode Require Import tactics.
 From iris.heap_lang Require Import proofmode notation.
-From iris.heap_lang Require Export lifting heap notation.
+From iris.heap_lang Require Export lifting notation.
 From iris.heap_lang.lib Require Import par.
-From iris.program_logic Require Import cancelable_invariants.
+From iris.base_logic Require Import cancelable_invariants.
 Import uPred.
 
 From iris_spanning_tree Require Import graph mon.
@@ -28,29 +27,27 @@ Definition span : val :=
   | SOME "y" =>
     if: try_mark "y" then
       let: "e" := ! "y" in
-      let: "rs" := "span" (Fst (Snd "e")) || "span" (Snd (Snd "e")) in
+      let: "rs" := "span" (Fst (Snd "e")) ||| "span" (Snd (Snd "e")) in
       ((if: ~ (Fst "rs") then unmark_fst "y" else #())
          ;; if: ~ (Snd "rs") then unmark_snd "y" else #());; #true
     else
       #false
   end.
 
-Global Opaque try_mark unmark_fst unmark_snd.
-
 Section Helpers.
   Context `{heapG Σ, cinvG Σ, graphG Σ, spawnG Σ} (κ : gname).
 
   Lemma wp_try_mark g Mrk k q (x : loc) : x ∈ dom (gset _) g →
-    heap_ctx ★ graph_ctx κ g Mrk ★ own_graph q ∅ ★ cinv_own κ k
+    graph_ctx κ g Mrk ∗ own_graph q ∅ ∗ cinv_own κ k
     ⊢ WP (try_mark #x) {{ v,
-         (v = #true ★ (∃ u, (g !! x) = Some u ★ own_graph q (x [↦] u))
-          ★ is_marked x ★ cinv_own κ k)
-           ∨ (v = #false ★ own_graph q ∅ ★ is_marked x ★ cinv_own κ k)
+         (⌜v = #true⌝ ∗ (∃ u, ⌜(g !! x) = Some u⌝ ∗ own_graph q (x [↦] u))
+          ∗ is_marked x ∗ cinv_own κ k)
+           ∨ (⌜v = #false⌝ ∗ own_graph q ∅ ∗ is_marked x ∗ cinv_own κ k)
       }}.
   Proof.
-    iIntros (Hgx) "(#Hheap & #Hgr & Hx & key)".
+    iIntros (Hgx) "(#Hgr & Hx & key)".
     wp_let; wp_bind (! _)%E. unfold graph_ctx.
-    iVs (cinv_open with "Hgr key") as "(>Hinv & key & Hcl)"; first done.
+    iMod (cinv_open with "Hgr key") as "(>Hinv & key & Hcl)"; first done.
     unfold graph_inv at 2.
     iDestruct "Hinv" as (G) "(Hi1 & Hi2 & Hi3 & Hi4)".
     iDestruct (graph_open with "[Hi1 Hi3]") as
@@ -61,13 +58,11 @@ Section Helpers.
     iDestruct "Hil1" as %Hil1. iDestruct "Hil2" as %Hil2.
     iDestruct (graph_close with "[Hi3 Hil3 Hil4]") as "Hi3"; eauto.
     { iFrame. iExists _; eauto. iSplitR; eauto. iExists _; by iFrame. }
-    iVs ("Hcl" with "[Hi1 Hi2 Hi3 Hi4]") as "_".
+    iMod ("Hcl" with "[Hi1 Hi2 Hi3 Hi4]") as "_".
     { iNext. unfold graph_inv at 2. iExists _; iFrame; auto. }
-    iVsIntro.
-    destruct u as [u1 u2]; simpl. wp_bind (Fst _). iApply wp_fst; eauto.
-    { rewrite children_to_val_is_val; eauto. }
-    iNext; iVsIntro; wp_let.
-    iVs (cinv_open _ graphN with "Hgr key")
+    iModIntro. wp_proj. wp_let.
+    destruct u as [u1 u2]; simpl.
+    iMod (cinv_open _ graphN with "Hgr key")
       as "(>Hinv & key & Hclose)"; first done.
     unfold graph_inv at 2.
     iDestruct "Hinv" as (G') "(Hi1 & Hi2 & Hi3 & Hi4)".
@@ -84,28 +79,28 @@ Section Helpers.
       iDestruct (graph_close with "[Hi3 Hil3 Hil4]") as "Hi3";
       eauto.
       { iFrame. iExists _; eauto. iSplitR; eauto. by iExists _; iFrame. }
-      iVs (already_marked with "Hi2") as "[Hi2 Hxm]"; [|iFrame "Hxm"].
+      iMod (already_marked with "Hi2") as "[Hi2 Hxm]"; [|iFrame "Hxm"].
       { by eapply in_dom_of_graph. }
-      iVs ("Hclose" with "[Hi1 Hi2 Hi3]") as "_".
+      iMod ("Hclose" with "[Hi1 Hi2 Hi3]") as "_".
       { iNext. unfold graph_inv at 2. iExists _; iFrame; auto. }
-      iVsIntro. iFrame. iRight; by iFrame.
+      iModIntro. iFrame. iRight; by iFrame.
     - (* CAS succeeds *)
       wp_cas_suc; first done.
-      iVs (mark_graph _ _ x uch with "[Hi1 Hx]") as "[Hi1 Hx]"; try by iFrame.
+      iMod (mark_graph _ _ x uch with "[Hi1 Hx]") as "[Hi1 Hx]"; try by iFrame.
       { apply (proj1 (not_elem_of_dom (D := gset loc) G' x)).
         intros Hid. eapply in_dom_of_graph in Hid; eauto; tauto. }
-      iVs (new_marked with "Hi2") as "[Hi2 Hm]". iFrame "key Hm".
+      iMod (new_marked with "Hi2") as "[Hi2 Hm]". iFrame "key Hm".
       erewrite delete_marked.
       iDestruct (auth_own_graph_valid with "Hi1") as %Hvl'.
       iDestruct (graph_close with "[Hi3 Hil3 Hil4]") as "Hi3".
       { iFrame. iExists (_, _). iSplitR; [| iExists _; iFrame]; trivial.
           rewrite mark_update_lookup; eauto. }
-      iVs ("Hclose" with "[Hi1 Hi2 Hi3]") as "_".
+      iMod ("Hclose" with "[Hi1 Hi2 Hi3]") as "_".
       + iNext; unfold graph_inv at 2. iExists _; iFrame.
         rewrite dom_op dom_singleton_L ?gset_op_union (comm union); iFrame.
         iPureIntro.
         { by apply mark_strict_subgraph. }
-      + iVsIntro. iLeft; iSplit; trivial. iExists _; iFrame.
+      + iModIntro. iLeft; iSplit; trivial. iExists _; iFrame.
         iPureIntro; eapply of_graph_unmarked; eauto.
   Qed.
 
@@ -121,18 +116,18 @@ Section Helpers.
 
   Lemma wp_load_graph g markings k q (x : loc) u w :
     (g !! x) = Some u →
-    (heap_ctx ★ graph_ctx κ g markings ★ own_graph q (x [↦] w) ★ cinv_own κ k)
+    (graph_ctx κ g markings ∗ own_graph q (x [↦] w) ∗ cinv_own κ k)
       ⊢
       WP (! #x)
-      {{ v, (∃ m : loc, (markings !! x) = Some m ∧
-              v = (#m, children_to_val w)%V) ★ ■ strict_sub_children u w
-              ★ own_graph q (x [↦] w) ★ cinv_own κ k }}.
+      {{ v, (∃ m : loc, ⌜markings !! x = Some m⌝ ∧
+              ⌜v = (#m, children_to_val w)⌝%V) ∗ ⌜strict_sub_children u w⌝
+              ∗ own_graph q (x [↦] w) ∗ cinv_own κ k }}.
   Proof.
-    iIntros (Hgx) "(#Hheap & #Hgr & Hx & key)".
+    iIntros (Hgx) "(#Hgr & Hx & key)".
     assert (Hgx' : x ∈ dom (gset _) g).
     { rewrite elem_of_dom Hgx; eauto. }
     unfold graph_ctx.
-    iVs (cinv_open _ graphN with "Hgr key")
+    iMod (cinv_open _ graphN with "Hgr key")
       as "(>Hinv & key & Hclose)"; first done.
     unfold graph_inv at 2.
     iDestruct "Hinv" as (G) "(Hi1 & Hi2 & Hi3 & Hi4)".
@@ -149,10 +144,10 @@ Section Helpers.
     rewrite mark_update_lookup in Hil1'; trivial.
     iDestruct (graph_close with "[Hi3 Hil3 Hil4]") as "Hi3"; [iFrame|].
     { iExists _; iSplitR; auto. iExists _; by iFrame. }
-    iVs ("Hclose" with "[Hi1 Hi2 Hi3]") as "_".
+    iMod ("Hclose" with "[Hi1 Hi2 Hi3]") as "_".
     { iNext. unfold graph_inv at 2. iExists _; iFrame; auto. }
     iFrame. inversion Hil1'; subst u'; simpl.
-    iVsIntro. iSplit; [|iPureIntro]. iExists _; iSplit; iPureIntro; eauto.
+    iModIntro. iSplit; [|iPureIntro]. iExists _; iSplit; iPureIntro; eauto.
     { rewrite Heq in Hi4. eapply laod_strict_sub_children; eauto. }
   Qed.
 
@@ -160,16 +155,16 @@ Section Helpers.
         (w w' : option loc * option loc) {m : loc} :
     strict_sub_children w w' → (markings !! x) = Some m →
       (g !! x) = Some v →
-      (heap_ctx ★ graph_ctx κ g markings ★ own_graph q (x [↦] w) ★ cinv_own κ k)
+      (graph_ctx κ g markings ∗ own_graph q (x [↦] w) ∗ cinv_own κ k)
         ⊢
         WP (#x <- (#m, children_to_val w'))
-        {{ v, own_graph q (x [↦] w') ★ cinv_own κ k }}.
+        {{ v, own_graph q (x [↦] w') ∗ cinv_own κ k }}.
   Proof.
-    iIntros (Hagree Hmrk Hgx) "(#Hheap & #Hgr & Hx & key)".
+    iIntros (Hagree Hmrk Hgx) "(#Hgr & Hx & key)".
     assert (Hgx' : x ∈ dom (gset _) g).
     { rewrite elem_of_dom Hgx; eauto. }
     unfold graph_ctx.
-    iVs (cinv_open _ graphN with "Hgr key")
+    iMod (cinv_open _ graphN with "Hgr key")
       as "(>Hinv & key & Hclose)"; first done.
     unfold graph_inv at 2.
     iDestruct "Hinv" as (G) "(Hi1 & Hi2 & Hi3 & Hi4)".
@@ -186,7 +181,7 @@ Section Helpers.
     pose proof Hil1 as Hil1'. rewrite Heq in Hil1' Hvl Hi4.
     rewrite mark_update_lookup in Hil1'; trivial. inversion Hil1'; subst u'.
     clear Hil1'. simpl. rewrite Heq.
-    iVs (update_graph _ _ _ w' with "[Hi1 Hx]") as
+    iMod (update_graph _ _ _ w' with "[Hi1 Hx]") as
         "[Hi1 Hx]"; try by iFrame. by rewrite lookup_delete.
     rewrite -delete_marked. erewrite (delete_marked _ _ _ w').
     assert (HvG : ✓ ({[x := Excl w']} ⋅ delete x G)).
@@ -194,7 +189,7 @@ Section Helpers.
     iDestruct (graph_close with "[Hi3 Hil3 Hil4]") as "Hi3".
     { iFrame. iExists _. iSplitR.
       - rewrite ?mark_update_lookup; eauto. - iExists _; by iFrame. }
-    iVs ("Hclose" with "[Hi1 Hi2 Hi3]") as "_"; [|by iFrame].
+    iMod ("Hclose" with "[Hi1 Hi2 Hi3]") as "_"; [|by iFrame].
     unfold graph_inv at 2.
     iNext. iExists _; iFrame. rewrite !dom_op !dom_singleton_L. iFrame.
     iPureIntro.
@@ -203,55 +198,41 @@ Section Helpers.
 
   Lemma wp_unmark_fst g markings k q (x : loc) v w1 w2 :
     (g !! x) = Some v →
-    (heap_ctx ★ graph_ctx κ g markings ★ own_graph q (x [↦] (w1, w2))
-     ★ cinv_own κ k) ⊢
+    (graph_ctx κ g markings ∗ own_graph q (x [↦] (w1, w2))
+     ∗ cinv_own κ k) ⊢
       WP (unmark_fst #x)
-      {{ _, own_graph q (x [↦] (None, w2)) ★ cinv_own κ k }}.
+      {{ _, own_graph q (x [↦] (None, w2)) ∗ cinv_own κ k }}.
   Proof.
-    iIntros (Hgx) "(#Hheap & #Hgr & Hx & key)".
+    iIntros (Hgx) "(#Hgr & Hx & key)".
     wp_let. wp_bind (! _)%E.
     iApply wp_wand_l; iSplitR;
-      [|iApply wp_load_graph; eauto; iFrame "Hheap Hgr"; by iFrame].
+      [|iApply wp_load_graph; eauto; iFrame "Hgr"; by iFrame].
     iIntros (u) "(H1 & Hagree & Hx & key)". iDestruct "H1" as (m) "[Hmrk Hu]".
     iDestruct "Hagree" as %Hagree.
     iDestruct "Hmrk" as %Hmrk; iDestruct "Hu" as %Hu; subst.
-    wp_let. wp_bind (Fst _). iApply wp_fst; eauto.
-    { rewrite children_to_val_is_val ; eauto. }
-    iNext; iVsIntro. wp_bind (Snd (_, _)). iApply wp_snd; eauto.
-    { by rewrite children_to_val_is_val. }
-    iNext; iVsIntro. wp_bind (Snd _). iApply wp_snd; eauto.
-    { rewrite to_of_val; eauto. }
-    {by rewrite to_of_val. }
-    iNext. iVsIntro.
+    wp_let. wp_bind (Fst _). do 3 wp_proj.
     iApply (wp_store_graph _ (None, w2) with "[Hx key]"); eauto;
-      [|iFrame "Hheap Hgr"; by iFrame].
+      [|iFrame "Hgr"; by iFrame].
     { by destruct w1; destruct w2; destruct v; inversion Hagree; subst. }
   Qed.
 
   Lemma wp_unmark_snd g markings k q (x : loc) v w1 w2 :
     (g !! x) = Some v →
-    (heap_ctx ★ graph_ctx κ g markings ★ own_graph q (x [↦] (w1, w2))
-     ★ cinv_own κ k) ⊢
+    (graph_ctx κ g markings ∗ own_graph q (x [↦] (w1, w2))
+     ∗ cinv_own κ k) ⊢
       WP (unmark_snd #x)
-      {{ _, own_graph q (x [↦] (w1, None)) ★ cinv_own κ k }}.
+      {{ _, own_graph q (x [↦] (w1, None)) ∗ cinv_own κ k }}.
   Proof.
-    iIntros (Hgx) "(#Hheap & #Hgr & Hx & key)".
+    iIntros (Hgx) "(#Hgr & Hx & key)".
     wp_let. wp_bind (! _)%E.
     iApply wp_wand_l; iSplitR;
-      [|iApply wp_load_graph; eauto; iFrame "Hheap Hgr"; by iFrame].
+      [|iApply wp_load_graph; eauto; iFrame "Hgr"; by iFrame].
     iIntros (u) "(H1 & Hagree & Hx & key)". iDestruct "H1" as (m) "[Hmrk Hu]".
     iDestruct "Hagree" as %Hagree.
     iDestruct "Hmrk" as %Hmrk; iDestruct "Hu" as %Hu; subst.
-    wp_let. wp_bind (Fst _). iApply wp_fst; eauto.
-    { rewrite children_to_val_is_val; eauto. }
-    iNext; iVsIntro. wp_bind (Snd (_, _)). iApply wp_snd; eauto.
-    { by rewrite children_to_val_is_val. }
-    iNext; iVsIntro. wp_bind (Fst _). iApply wp_fst; eauto.
-    {by rewrite to_of_val. }
-    { rewrite to_of_val; eauto. }
-    iNext. iVsIntro.
+    wp_let. wp_bind (Fst _). do 3 wp_proj.
     iApply (wp_store_graph _ (w1, None) with "[Hx key]"); eauto;
-      [|iFrame "Hheap Hgr"; by iFrame].
+      [|iFrame "Hgr"; by iFrame].
     { by destruct w1; destruct w2; destruct v; inversion Hagree; subst. }
   Qed.
 
@@ -267,7 +248,7 @@ Section Helpers.
     g !! l = Some (u1, u2) →
     match u1 with |Some l1 => l1 ∈ t | None => True end →
     match u2 with |Some l2 => l2 ∈ t | None => True end →
-    front g (dom (gset _) (l [↦] w)) t.
+    front g (dom (gset loc) (l [↦] w : gmap loc _)) t.
   Proof.
     intros Hgl Hu1 Hu2.
     split => [x |x y]; rewrite ?dom_singleton ?elem_of_singleton => ?; subst.
@@ -276,7 +257,7 @@ Section Helpers.
       destruct u1; destruct u2; simpl; intros [Heq|Heq]; by inversion Heq; subst.
   Qed.
   Lemma empty_graph_divide q :
-    own_graph q ∅ ⊢ own_graph (q / 2) ∅ ★ own_graph (q / 2) ∅.
+    own_graph q ∅ ⊢ own_graph (q / 2) ∅ ∗ own_graph (q / 2) ∅.
   Proof.
     setoid_replace (∅ : gmapR loc (exclR chlC)) with
     (∅ ⋅ ∅ : gmapR loc (exclR chlC)) at 1 by (by rewrite ucmra_unit_left_id).
@@ -286,11 +267,11 @@ Section Helpers.
   Lemma front_marked (g : graph loc) (l : loc) u1 u2 w mr1 mr2 (G1 G2 : Gmon) :
     g !! l = Some (u1, u2) →
     (front g (dom (gset _) G1) mr1) → (front g (dom (gset _) G2) mr2) →
-    ([★ set] l ∈ mr1, is_marked l) ★ ([★ set] l ∈ mr2, is_marked l) ★
-    match u1 with |Some l1 => is_marked l1 | None => True end ★
+    ([∗ set] l ∈ mr1, is_marked l) ∗ ([∗ set] l ∈ mr2, is_marked l) ∗
+    match u1 with |Some l1 => is_marked l1 | None => True end ∗
     match u2 with |Some l2 => is_marked l2 | None => True end ⊢
-    ∃ (mr : gset loc), ■ front g (dom (gset loc) ((l [↦] w) ⋅ (G1 ⋅ G2))) mr
-      ★ ([★ set] l ∈ mr, is_marked l).
+    ∃ (mr : gset loc), ⌜front g (dom (gset loc) ((l [↦] w) ⋅ (G1 ⋅ G2))) mr⌝
+      ∗ ([∗ set] l ∈ mr, is_marked l).
   Proof.
     iIntros (Hgl Hfr1 Hfr2) "(Hmr1 & Hmr2 & Hu1 & Hu2)".
     iExists (match u1 with |Some l1 => {[l1]} | None => ∅ end ∪
@@ -310,27 +291,27 @@ Section Helpers.
     maximal g →
     (x = NONEV ∨ ∃ l : loc,
         x = SOMEV #l ∧ l ∈ dom (gset _) g) →
-    (heap_ctx ★ graph_ctx κ g markings ★ own_graph q ∅ ★ cinv_own κ k)
+    (graph_ctx κ g markings ∗ own_graph q ∅ ∗ cinv_own κ k)
       ⊢
       WP (span x)
-      {{ v, ((v = # true ★
-             (∃ l : loc, x = SOMEV #l ★
+      {{ v, ((⌜v = # true⌝ ∗
+             (∃ l : loc, ⌜x = SOMEV #l⌝ ∗
                (∃ (G : Gmon) mr (tr : tree (Gmon_graph G) l),
-                  own_graph q G ★ ■ (l ∈ dom (gset _) G) ★
-                  ■ maximal (Gmon_graph G) ★ ■ (front g (dom (gset _) G) mr) ★
-                   ([★ set] l ∈ mr , is_marked l)) ★ is_marked l)) ∨
-             (v = # false ★
-              (x = NONEV ∨ (∃ l : loc, x = SOMEV #l ★ is_marked l))
-               ★ own_graph q ∅))
-            ★ cinv_own κ k
+                  own_graph q G ∗ ⌜l ∈ dom (gset _) G⌝ ∗
+                  ⌜maximal (Gmon_graph G)⌝ ∗ ⌜front g (dom (gset _) G) mr⌝ ∗
+                   ([∗ set] l ∈ mr , is_marked l)) ∗ is_marked l)) ∨
+             (⌜v = # false⌝ ∗
+              (⌜x = NONEV⌝ ∨ (∃ l : loc, ⌜x = SOMEV #l⌝ ∗ is_marked l))
+               ∗ own_graph q ∅))
+            ∗ cinv_own κ k
       }}.
   Proof.
-    intros [_ Hgmx] Hxpt. iIntros "(#Hheap & #Hgr & Hx & key)".
+    intros [_ Hgmx] Hxpt. iIntros "(#Hgr & Hx & key)".
     iRevert (x Hxpt k q) "key Hx". iLöb as "IH".
     iIntros (x Hxpt k q) "key Hx".
     wp_rec.
     destruct Hxpt as [|[l [? Hgsl]]]; subst.
-    { wp_match. iVsIntro.
+    { wp_match.
       iFrame; iRight; iFrame; repeat iSplit; trivial; by iLeft. }
     wp_match. wp_bind (try_mark _).
     iDestruct (empty_graph_divide with "Hx") as "[Hx1 Hx2]".
@@ -338,63 +319,47 @@ Section Helpers.
       [|iApply wp_try_mark; try iFrame]; eauto; simpl.
     iIntros (v) "[(% & Hv & Hm & key)|(% & Hx2 & Hm & key)]"; subst;
     [|iCombine "Hx1" "Hx2" as "Hx"; rewrite -graph_divide ucmra_unit_right_id;
-      wp_if; iVsIntro; iFrame; iRight; iFrame; iSplit; trivial; iRight;
+      wp_if; iFrame; iRight; iFrame; iSplit; trivial; iRight;
       iExists _; eauto].
     iDestruct "Hv" as (u) "[Hgl Hl]". iDestruct "Hgl" as %Hgl.
     wp_if.
     (* reading the reference. This part is very similar to unmark lemmas! *)
     wp_bind (! _)%E.
     iApply wp_wand_l; iSplitR "Hl key";
-      [|iApply wp_load_graph; eauto; iFrame "Hheap Hgr"; by iFrame].
+      [|iApply wp_load_graph; eauto; iFrame "Hgr"; by iFrame].
     iIntros (v) "(H1 & Hagree & Hx & key)". iDestruct "H1" as (m) "[Hmrk Hv]".
     iDestruct "Hagree" as %Hagree. iDestruct "Hv" as %Hv; subst v.
     wp_let. wp_bind (par _).
-    erewrite <- cinv_own_half. iDestruct "key" as "[K1 K2]".
+    iDestruct "key" as "[K1 K2]".
     iDestruct (empty_graph_divide with "Hx1") as "[Hx11 Hx12]".
-    destruct u as [u1 u2]. iApply wp_par. iSplitR; [by iFrame "Hheap"|].
+    destruct u as [u1 u2]. iApply (par_spec with "[Hx11 K1] [Hx12 K2]").
     (* symbolically executing the left part of the par. *)
-    iSplitL "Hx11 K1".
-    wp_bind (Snd _). iApply wp_snd; eauto.
-    { by rewrite children_to_val_is_val. }
-    iNext; iVsIntro. wp_bind (Fst _). iApply wp_fst.
-    { by rewrite to_of_val. }
-    { rewrite to_of_val; eauto. }
-    iNext; iVsIntro.
-    assert (Hlf : (child_to_val u1) = NONEV
-                ∨ (∃ l : loc,
-                      (child_to_val u1) = SOMEV #l ∧ l ∈ dom (gset _) g)).
+    wp_lam; repeat wp_proj.
+    assert ((child_to_val u1) = NONEV
+            ∨ (∃ l : loc,
+                  (child_to_val u1) = SOMEV #l ∧ l ∈ dom (gset _) g)) as Hlf.
     { destruct u1 as [l1|]; [right |by left].
       exists l1; split; trivial. eapply (Hgmx l); rewrite // /get_left Hgl; auto. }
     iApply ("IH" with "[#] * [K1] [Hx11]"); auto.
     (* symbolically executing the left part of the par. *)
-    iSplitL "Hx12 K2".
-    wp_bind (Snd (_, _)). iApply wp_snd; eauto.
-    { by rewrite children_to_val_is_val. }
-    iNext; iVsIntro. wp_bind (Snd _). iApply wp_snd.
-    { rewrite to_of_val; eauto. }
-    { by rewrite to_of_val. }
-    iNext; iVsIntro.
-    assert (Hrh : (child_to_val u2) = NONEV
+    wp_lam; repeat wp_proj.
+    assert ((child_to_val u2) = NONEV
                 ∨ (∃ l : loc,
-                      (child_to_val u2) = SOMEV #l ∧ l ∈ dom (gset _) g)).
+                      (child_to_val u2) = SOMEV #l ∧ l ∈ dom (gset _) g)) as Hrh.
     { destruct u2 as [l2|]; [right |by left].
       exists l2; split; trivial. eapply (Hgmx l); rewrite // /get_right Hgl; auto. }
     iApply ("IH" with "[#] * [K2] [Hx12]"); auto.
-    iIntros (vl vr) "[[Hvl K1] [Hvr K2]]".
-    iCombine "K1" "K2" as "key". rewrite cinv_own_half.
+    (* continuing after both children are processed *)
+    iNext.
+    iIntros (vl vr) "([Hvl K1] & Hvr & K2 & K2')".
+    iCombine "K2" "K2'" as "K2". iCombine "K1" "K2" as "key".
     iNext. wp_let.
     (* We don't need the huge induction hypothesis anymore. *)
     iClear "IH".
     (* separating all four cases *)
     iDestruct "Hvl" as "[[% Hvll]|[% Hvlr]]"; subst;
       iDestruct "Hvr" as "[[% Hvrl]|[% Hvrr]]"; subst.
-    - wp_bind (Fst _). iApply wp_fst; eauto. iNext; iVsIntro.
-      wp_bind (UnOp _ _). iApply wp_un_op; try done. iNext; iVsIntro.
-      wp_if; wp_seq.
-      wp_bind (Snd _). iApply wp_snd; eauto. iNext; iVsIntro.
-      wp_bind (UnOp _ _). iApply wp_un_op; try done.
-      iNext; iVsIntro.
-      wp_if.
+    - wp_proj. wp_op. wp_if; wp_seq. wp_proj. wp_op. wp_if. wp_seq.
       iDestruct "Hvll" as (l1) "(Hl1eq & Hg1 & ml1)".
       iDestruct "Hg1" as (G1 mr1 tr1) "(Hxl & Hl1im & Hmx1 & Hfr1 & Hfml)".
       iDestruct "Hfr1" as %Hfr1. iDestruct "Hmx1" as %Hmx1.
@@ -406,7 +371,7 @@ Section Helpers.
       iCombine "Hxl" "Hxr" as "Hxlr". rewrite -graph_divide.
       iCombine "Hx" "Hxlr" as "Hx". rewrite -graph_divide.
       destruct u1; destruct u2; inversion Hl1eq; inversion Hl2eq; subst.
-      iVsIntro. iFrame; iLeft. iSplit; [trivial|].
+      iFrame; iLeft. iSplit; [trivial|].
       iExists _; iSplit; [trivial|]. iFrame.
       iDestruct (own_graph_valid with "Hx") as %Hvl.
       iExists ({[l := Excl (Some l1, Some l2)]} ⋅ (G1 ⋅ G2)).
@@ -414,27 +379,23 @@ Section Helpers.
       "[ml1 ml2 Hfml Hfmr]") as (mr)"[Hfr Hfm]"; eauto. iDestruct "Hfr" as %Hfr.
       iExists mr.
       unshelve iExists _; [eapply maximally_marked_tree_both; eauto|].
-      iFrame. repeat iSplit; try iPureIntro; eauto.
+      iFrame. iSplit; try iPureIntro; eauto.
       { rewrite dom_op dom_singleton elem_of_union elem_of_singleton; by left. }
+      split; auto.
       { eapply maximally_marked_tree_both; eauto. }
-    - wp_bind (Fst _). iApply wp_fst; eauto. iNext; iVsIntro.
-      wp_bind (UnOp _ _). iApply wp_un_op; try done. iNext; iVsIntro.
-      wp_if; wp_seq.
-      wp_bind (Snd _). iApply wp_snd; eauto. iNext; iVsIntro.
-      wp_bind (UnOp _ _). iApply wp_un_op; try done.
-      iNext; iVsIntro.
-      wp_if.
+    - wp_proj. wp_op. wp_if. wp_seq. wp_proj. wp_op. wp_if.
       iDestruct "Hvll" as (l1) "(Hl1eq & Hg1 & ml1)".
       iDestruct "Hg1" as (G1 mr1 tr1) "(Hxl & Hl1im & Hmx1 & Hfr1 & Hfml)".
       iDestruct "Hfr1" as %Hfr1. iDestruct "Hmx1" as %Hmx1.
       iDestruct "Hl1eq" as %Hl1eq. iDestruct "Hl1im" as %Hl1im.
       iDestruct "Hvrr" as "(Hvr & Hxr)".
       iCombine "Hxl" "Hxr" as "Hxlr". rewrite -graph_divide ucmra_unit_right_id.
+      wp_bind (unmark_snd _).
       iApply wp_wand_l; iSplitR "Hx key";
-        [|iApply wp_unmark_snd; eauto; by iFrame "Hgr Hheap"; iFrame].
+        [|iApply wp_unmark_snd; eauto; by iFrame "Hgr"; iFrame].
       iIntros (v) "[Hx key]".
       iCombine "Hx" "Hxlr" as "Hx". rewrite -graph_divide.
-      wp_value; iVsIntro; wp_seq; iVsIntro.
+      wp_seq.
       iFrame; iLeft. iSplit; [trivial|].
       iExists _; iSplit; [trivial|]. iFrame.
       iDestruct (own_graph_valid with "Hx") as %Hvld.
@@ -451,28 +412,23 @@ Section Helpers.
       iDestruct "Hfr" as %Hfr. rewrite right_id_L in Hfr.
       iExists mr.
       unshelve iExists _; [eapply maximally_marked_tree_left; eauto|].
-      iFrame. repeat iSplit; try iPureIntro; eauto.
+      iFrame. iSplit; try iPureIntro; eauto.
       { rewrite dom_op dom_singleton elem_of_union elem_of_singleton; by left. }
+      split; auto.
       { eapply maximally_marked_tree_left; eauto. }
-    - wp_bind (Fst _). iApply wp_fst; eauto. iNext; iVsIntro.
-      wp_bind (UnOp _ _). iApply wp_un_op; try done. iNext; iVsIntro.
-      wp_if.
+    - wp_proj. wp_op. wp_if.
       iDestruct "Hvlr" as "(Hvl & Hxl)".
       iDestruct "Hvrl" as (l2) "(Hl2eq & Hg2 & ml2)".
       iDestruct "Hg2" as (G2 mr2 tr2) "(Hxr & Hl2im & Hmx2 & Hfr2 & Hfmr)".
       iDestruct "Hfr2" as %Hfr2. iDestruct "Hmx2" as %Hmx2.
       iDestruct "Hl2eq" as %Hl2eq. iDestruct "Hl2im" as %Hl1im.
       iCombine "Hxl" "Hxr" as "Hxlr". rewrite -graph_divide left_id.
+      wp_bind (unmark_fst _).
       iApply wp_wand_l; iSplitR "Hx key";
-        [|iApply wp_unmark_fst; eauto; by iFrame "Hgr Hheap"; iFrame].
+        [|iApply wp_unmark_fst; eauto; by iFrame "Hgr"; iFrame].
       iIntros (v) "[Hx key]".
       iCombine "Hx" "Hxlr" as "Hx". rewrite -graph_divide.
-      wp_seq.
-      wp_bind (Snd _). iApply wp_snd; eauto. iNext; iVsIntro.
-      wp_bind (UnOp _ _). iApply wp_un_op; try done.
-      iNext; iVsIntro.
-      wp_if.
-      iVsIntro.
+      wp_seq. wp_proj. wp_op. wp_if. wp_seq.
       iFrame; iLeft. iSplit; [trivial|].
       iExists _; iSplit; [trivial|]. iFrame.
       iDestruct (own_graph_valid with "Hx") as %Hvld.
@@ -489,29 +445,23 @@ Section Helpers.
       iDestruct "Hfr" as %Hfr. rewrite left_id_L in Hfr.
       iExists mr.
       unshelve iExists _; [eapply maximally_marked_tree_right; eauto|].
-      iFrame. repeat iSplit; try iPureIntro; eauto.
+      iFrame. iSplit; try iPureIntro; eauto.
       { rewrite dom_op dom_singleton elem_of_union elem_of_singleton; by left. }
+      split; auto.
       { eapply maximally_marked_tree_right; eauto. }
     - iDestruct "Hvlr" as "(Hvl & Hxl)".
       iDestruct "Hvrr" as "(Hvr & Hxr)".
       iCombine "Hxl" "Hxr" as "Hxlr". rewrite -graph_divide ucmra_unit_right_id.
-      wp_bind (Fst _). iApply wp_fst; eauto. iNext; iVsIntro.
-      wp_bind (UnOp _ _). iApply wp_un_op; try done. iNext; iVsIntro.
-      wp_if.
+      wp_proj. wp_op. wp_if. wp_bind(unmark_fst _).
       iApply wp_wand_l; iSplitR "Hx key";
-        [|iApply wp_unmark_fst; eauto; by iFrame "Hgr Hheap"; iFrame].
+        [|iApply wp_unmark_fst; eauto; by iFrame "Hgr"; iFrame].
       iIntros (v) "[Hx key]".
-      wp_seq.
-      wp_bind (Snd _). iApply wp_snd; eauto. iNext; iVsIntro.
-      wp_bind (UnOp _ _). iApply wp_un_op; try done.
-      iNext; iVsIntro.
-      wp_if.
+      wp_seq. wp_proj. wp_op. wp_if. wp_bind(unmark_snd _).
       iApply wp_wand_l; iSplitR "Hx key";
-        [|iApply wp_unmark_snd; eauto; by iFrame "Hgr Hheap"; iFrame].
+        [|iApply wp_unmark_snd; eauto; by iFrame "Hgr"; iFrame].
       clear v. iIntros (v) "[Hx key]".
       iCombine "Hx" "Hxlr" as "Hx". rewrite -graph_divide.
       wp_seq.
-      iVsIntro.
       iFrame; iLeft. iSplit; [trivial|].
       iExists _; iSplit; [trivial|]. iFrame.
       iDestruct (own_graph_valid with "Hx") as %Hvld.
@@ -534,8 +484,9 @@ Section Helpers.
       iExists mr.
       rewrite right_id_L. rewrite right_id_L in Hvld Hfr.
       unshelve iExists _; [eapply maximally_marked_tree_none; eauto|].
-      iFrame. repeat iSplit; try iPureIntro; eauto.
+      iFrame. iSplit; try iPureIntro; eauto.
       { by rewrite dom_singleton elem_of_singleton. }
+      split; auto.
       { eapply maximally_marked_tree_none; eauto. }
   Qed.
 
